small fix; introduce IntoVecVal

theories/typing/cont.v
@@ -1,19 +1,28 @@
-From iris.proofmode Require Import tactics.
 From lrust.typing Require Export type.
 From lrust.typing Require Import programs.
 Set Default Proof Using "Type".
+
+Class IntoVecVal {n} (el: list expr) (vl: vec val n) :=
+  into_vec_val: el = map of_val vl.
+
+Global Instance into_vec_val_nil: IntoVecVal [] [#].
+Proof. done. Qed.
+
+Global Instance into_vec_val_cons {n} e v el (vl: _ n) :
+  IntoVal e v → IntoVecVal el vl → IntoVecVal (e :: el) (v ::: vl).
+Proof. by move=>/= <-->. Qed.
 
 Section typing.
   Context `{!typeG Σ}.
 
   (** Jumping to and defining a continuation. *)
-  Lemma type_jump {𝔄l 𝔅l} E (T: _ 𝔄l) C k L n (T': _ → _ 𝔅l) pre el (vl: vec _ n) tr :
-    k ◁cont{L, T'} pre ∈ C → el = map of_val vl → tctx_incl E L T (T' vl) tr →
+  Lemma type_jump {𝔄l 𝔅l n} E (T: _ 𝔄l) C k L (T': _ → _ 𝔅l) pre el (vl: _ n) tr :
+    IntoVecVal el vl → k ◁cont{L, T'} pre ∈ C → tctx_incl E L T (T' vl) tr →
     ⊢ typed_body E L C T (k el) (tr pre).
   Proof.
-    iIntros (InC -> TT' ??) "LFT _ PROPH UNIQ E Na L C T Obs".
+    move=> -> ?. iIntros (TT' ??) "LFT _ PROPH UNIQ E Na L C T Obs".
     iMod (TT' with "LFT PROPH UNIQ E L T Obs") as (?) "(L & T & Obs)".
-    iSpecialize ("C" with "[%//]"). iApply ("C" with "Na L T Obs").
+    iApply ("C" with "[%//] Na L T Obs").
   Qed.
 
   Lemma type_cont {𝔄l 𝔅l} E L C (T: _ 𝔄l) kb bl ec e L' (T': _ → _ 𝔅l) prek pre :
@@ -23,8 +32,8 @@ Section typing.
       (T' vl) (subst' kb k $ subst_v bl vl ec) prek) -∗
     typed_body E L C T (letcont: kb bl := ec in e) pre.
   Proof.
-    iIntros (??) "e #ec". iIntros (??) "#LFT #TIME #PROPH #UNIQ #E Na L C T Obs".
-    have ->: (rec: kb bl := ec)%E = of_val (rec: kb bl := ec) by unlock.
+    iIntros (??) "e #ec %% #LFT #TIME #PROPH #UNIQ #E Na L C T Obs".
+    have ->: (rec: kb bl := ec)%E = of_val (rec: _ _ := _) by unlock.
     wp_let. iApply ("e" with "LFT TIME PROPH UNIQ E Na L [C] T Obs").
     iLöb as "IH". iIntros (?). rewrite elem_of_cons.
     iIntros ([->|?]); [|by iApply "C"]. iIntros (??) "Na L' T' Obs".
@@ -39,12 +48,12 @@ Section typing.
       typed_body E L' C (T' vl) (subst' kb k $ subst_v bl vl ec) prek) -∗
     typed_body E L C T (letcont: kb bl := ec in e) pre.
   Proof.
-    iIntros (??) "e ec". iIntros (??) "#LFT #TIME #PROPH #UNIQ #E Na L C T Obs".
-    have ->: (rec: kb bl := ec)%E = of_val (rec: kb bl := ec) by unlock.
+    iIntros (??) "e ec %% #LFT #TIME #PROPH #UNIQ #E Na L C T Obs".
+    have ->: (rec: kb bl := ec)%E = of_val (rec: _ _ := _) by unlock.
     wp_let. iApply ("e" with "LFT TIME PROPH UNIQ E Na L [ec C] T Obs").
-    iIntros (?). rewrite elem_of_cons.
-    iIntros ([->|?]); [|by iApply "C"]. iIntros (??) "Na L' T' Obs".
-    wp_rec. by iApply ("ec" with "LFT TIME PROPH UNIQ E Na L' [C] T' Obs").
+    iIntros (?). rewrite elem_of_cons. iIntros ([->|?]); [|by iApply "C"].
+    iIntros (??) "Na L' T' Obs". wp_rec.
+    iApply ("ec" with "LFT TIME PROPH UNIQ E Na L' C T' Obs").
   Qed.
 
 End typing.
