theories/typing/borrow.v
@@ -1,5 +1,3 @@
-From iris.proofmode Require Import tactics.
-From lrust.lang Require Import proofmode.
 From lrust.typing Require Export uniq_bor shr_bor own.
 From lrust.typing Require Import lft_contexts type_context programs.
 Set Default Proof Using "Type".
